pickle-stubs/pipecat/serializers/livekit.pyi
@@ -1,9 +1,8 @@
 from typing import Any
 
 from _unsafe import Unsafe
+from pickle_stubs_secure.trust import TrustedBytes
 
 
 class LivekitFrameSerializer:
-    def deserialize(self, data: bytes, *args: Any, **kwargs: Any) -> Unsafe[Any]: ...
-    async def deserialize_async(self, data: bytes, *args: Any, **kwargs: Any) -> Unsafe[Any]: ...
-
+    async def deserialize(self, data: TrustedBytes, *args: Any, **kwargs: Any) -> Unsafe[Any]: ...
