stubs/torch_musa/utils/compare_tool.pyi
@@ -1,8 +1,20 @@
 from typing import Any
 
 from _unsafe import Unsafe
+from pickle_stubs_secure.trust import TrustedPath
 
 
-def compare_for_single_op(*args: Any, **kwargs: Any) -> Unsafe[Any]: ...
-def nan_inf_track_for_single_op(*args: Any, **kwargs: Any) -> Unsafe[Any]: ...
-
+def compare_for_single_op(
+    inputs_data_save_path: TrustedPath,
+    op_func: Any,
+    atol: float,
+    rtol: float,
+    *args: Any,
+    **kwargs: Any,
+) -> Unsafe[Any]: ...
+def nan_inf_track_for_single_op(
+    inputs_data_save_path: TrustedPath,
+    op_func: Any,
+    *args: Any,
+    **kwargs: Any,
+) -> Unsafe[Any]: ...
